src/lib/DenseOrder.v
@@ -24,7 +24,7 @@ Module Type IsDense (Import T:EqLtLe).
       lt (middle lhs rhs) rhs.
 End IsDense.
 
-Module Type DenseOrderType := UsualOrderedTypeFull <+ IsDense.
+Module Type DenseOrderType := UsualOrderedTypeFull <+ IsDense <+ HasCaseJoin.
 
 Module DenseOrder: DenseOrderType.
   Definition t := list bool.
@@ -138,6 +138,82 @@ Module DenseOrder: DenseOrderType.
       destruct a; econs; auto.
     - exploit IHlhs; eauto. i. des.
       destruct a; econs; auto.
+  Qed.
+
+  Lemma le_lt_dec (lhs rhs:t): {le lhs rhs} + {lt rhs lhs}.
+  Proof.
+    generalize (compare_spec lhs rhs).
+    destruct (compare lhs rhs).
+    - left. inv H. right. ss.
+    - left. inv H. apply le_lteq. auto.
+    - right. inv H. auto.
+  Defined.
+
+  Definition join (lhs rhs:t): t :=
+    if le_lt_dec lhs rhs
+    then rhs
+    else lhs.
+
+  Lemma join_comm lhs rhs: join lhs rhs = join rhs lhs.
+  Proof.
+    unfold join.
+    destruct (le_lt_dec lhs rhs), (le_lt_dec rhs lhs); auto.
+    - unfold le in *. des; auto.
+      rewrite l0 in l. apply lt_strorder in l. done.
+    - rewrite l0 in l. apply lt_strorder in l. done.
+  Qed.
+
+  Lemma join_assoc a b c: join (join a b) c = join a (join b c).
+  Proof.
+    unfold join.
+    repeat
+      (try match goal with
+           | [|- context[le_lt_dec ?a ?b]] =>
+             destruct (le_lt_dec a b)
+           | [H: context[le_lt_dec ?a ?b] |- _] =>
+             destruct (le_lt_dec a b)
+           | [H1: lt ?a ?b, H2: lt ?b ?a |- _] =>
+             rewrite H2 in H1; apply lt_strorder in H1; inv H1
+           end; unfold le, eq in *; try subst; des; ss).
+    - rewrite l in l2. rewrite l0 in l2.
+      apply lt_strorder in l2. inv l2.
+    - rewrite l in l2. rewrite l1 in l2.
+      apply lt_strorder in l2. inv l2.
+  Qed.
+
+  Lemma join_l lhs rhs:
+    le lhs (join lhs rhs).
+  Proof.
+    unfold join. destruct (le_lt_dec lhs rhs); auto.
+    apply le_lteq. auto.
+  Qed.
+
+  Lemma join_r lhs rhs:
+    le rhs (join lhs rhs).
+  Proof.
+    rewrite join_comm. apply join_l.
+  Qed.
+
+  Lemma join_spec lhs rhs o
+        (LHS: le lhs o)
+        (RHS: le rhs o):
+    le (join lhs rhs) o.
+  Proof.
+    unfold join. destruct (le_lt_dec lhs rhs); auto.
+  Qed.
+
+  Lemma join_spec_lt lhs rhs o
+        (LHS: lt lhs o)
+        (RHS: lt rhs o):
+    lt (join lhs rhs) o.
+  Proof.
+    unfold join. destruct (le_lt_dec lhs rhs); auto.
+  Qed.
+
+  Lemma join_cases lhs rhs:
+    join lhs rhs = lhs \/ join lhs rhs = rhs.
+  Proof.
+    unfold join. destruct (le_lt_dec lhs rhs); auto.
   Qed.
 End DenseOrder.
 
